Fix and add weakest under approximate post
still a problem with Kleene star semantics

.Makefile.d
@@ -1,10 +1,8 @@
-theories/StateMap.vo theories/StateMap.glob theories/StateMap.v.beautified theories/StateMap.required_vo: theories/StateMap.v 
-theories/StateMap.vos theories/StateMap.vok theories/StateMap.required_vos: theories/StateMap.v 
-theories/Imp.vo theories/Imp.glob theories/Imp.v.beautified theories/Imp.required_vo: theories/Imp.v theories/StateMap.vo
-theories/Imp.vos theories/Imp.vok theories/Imp.required_vos: theories/Imp.v theories/StateMap.vos
-theories/Hoare.vo theories/Hoare.glob theories/Hoare.v.beautified theories/Hoare.required_vo: theories/Hoare.v theories/StringAsOT.vo theories/StateMap.vo theories/Imp.vo
-theories/Hoare.vos theories/Hoare.vok theories/Hoare.required_vos: theories/Hoare.v theories/StringAsOT.vos theories/StateMap.vos theories/Imp.vos
-theories/Inc.vo theories/Inc.glob theories/Inc.v.beautified theories/Inc.required_vo: theories/Inc.v theories/StringAsOT.vo theories/StateMap.vo theories/Imp.vo theories/Hoare.vo
-theories/Inc.vos theories/Inc.vok theories/Inc.required_vos: theories/Inc.v theories/StringAsOT.vos theories/StateMap.vos theories/Imp.vos theories/Hoare.vos
-theories/StringAsOT.vo theories/StringAsOT.glob theories/StringAsOT.v.beautified theories/StringAsOT.required_vo: theories/StringAsOT.v 
-theories/StringAsOT.vos theories/StringAsOT.vok theories/StringAsOT.required_vos: theories/StringAsOT.v 
+theories/StateMap.vo theories/StateMap.glob theories/StateMap.v.beautified theories/StateMap.required_vo: theories/StateMap.v /Users/alessiocoltellacci/.opam/5.0.0/lib/rocq-runtime/rocqworker
+theories/StateMap.vos theories/StateMap.vok theories/StateMap.required_vos: theories/StateMap.v /Users/alessiocoltellacci/.opam/5.0.0/lib/rocq-runtime/rocqworker
+theories/Imp.vo theories/Imp.glob theories/Imp.v.beautified theories/Imp.required_vo: theories/Imp.v theories/StateMap.vo /Users/alessiocoltellacci/.opam/5.0.0/lib/rocq-runtime/rocqworker
+theories/Imp.vos theories/Imp.vok theories/Imp.required_vos: theories/Imp.v theories/StateMap.vos /Users/alessiocoltellacci/.opam/5.0.0/lib/rocq-runtime/rocqworker
+theories/Hoare.vo theories/Hoare.glob theories/Hoare.v.beautified theories/Hoare.required_vo: theories/Hoare.v theories/Imp.vo theories/StateMap.vo /Users/alessiocoltellacci/.opam/5.0.0/lib/rocq-runtime/rocqworker
+theories/Hoare.vos theories/Hoare.vok theories/Hoare.required_vos: theories/Hoare.v theories/Imp.vos theories/StateMap.vos /Users/alessiocoltellacci/.opam/5.0.0/lib/rocq-runtime/rocqworker
+theories/Inc.vo theories/Inc.glob theories/Inc.v.beautified theories/Inc.required_vo: theories/Inc.v theories/Imp.vo theories/StateMap.vo /Users/alessiocoltellacci/.opam/5.0.0/lib/rocq-runtime/rocqworker
+theories/Inc.vos theories/Inc.vok theories/Inc.required_vos: theories/Inc.v theories/Imp.vos theories/StateMap.vos /Users/alessiocoltellacci/.opam/5.0.0/lib/rocq-runtime/rocqworker
