theories/Imp.v
@@ -1,10 +1,18 @@
-Require Export Coq.Strings.String.
+From Coq Require Import Strings.String Bool.
 Require Import StateMap.
+
+Local Open Scope string_scope.
+Local Open Scope Z_scope.
+Local Open Scope list_scope.
+
+Definition ident := string.
 
 Inductive aexp : Type :=
   | ANum (n : nat)
-  | AId (x : string)
+  | AId (x : ident)
   | APlus (a1 a2 : aexp)
+  | AMinus (a1 a2 : aexp)
+  | AMult (a1 a2 : aexp)
 .
 
 Inductive bexp : Type :=
@@ -12,6 +20,8 @@ Inductive bexp : Type :=
   | BFalse
   | BEq (a1 a2 : aexp)
   | BNot (b : bexp)
+  | BLessEqual (a1 a2 : aexp)
+  | BAnd (a1 a2 : bexp)
 .
 
 Inductive com : Type :=
@@ -20,16 +30,19 @@ Inductive com : Type :=
   | Seq : com -> com -> com
   | Assume : bexp -> com
   | Error: com
-  | Star: com -> com
-  | Choice: com -> com -> com
-  | CLocal: string -> com -> com.
+  | Star: com -> com                   (* Kleene iteration *)
+  | Choice: com -> com -> com          (* Kleene algebra union *)
+  | CLocal: string -> com -> com
+  | Nondet: string -> com.             (* Nondet Assignment *)
 
-Coercion AId : string >-> aexp.
+Coercion AId : ident >-> aexp.
 
 Coercion ANum : nat >-> aexp.
 
 Declare Custom Entry com.
+
 Declare Scope com_scope.
+
 Notation "<{ e }>" := e (at level 0, e custom com at level 99) : com_scope.
 Notation "( x )" := x (in custom com, x at level 99) : com_scope.
 Notation "x" := x (in custom com at level 0, x constr at level 0) : com_scope.
@@ -37,12 +50,17 @@ Notation "f x .. y" := (.. (f x) .. y)
                   (in custom com at level 0, only parsing,
                   f constr at level 0, x constr at level 9,
                   y constr at level 9) : com_scope.
-Notation "x + y" := (APlus x y) (in custom com at level 50, left associativity).
+Notation "x + y" := (APlus x y) (in custom com at level 70, left associativity).
+Notation "x - y" := (AMinus x y) (in custom com at level 70, left associativity).
+Notation "x * y" := (AMult x y) (in custom com at level 50, left associativity).
 Notation "'true'" := true (at level 1).
 Notation "'true'" := BTrue (in custom com at level 0).
 Notation "'false'" := false (at level 1).
 Notation "'false'" := BFalse (in custom com at level 0).
 Notation "x = y" := (BEq x y) (in custom com at level 70, no associativity).
+Notation "'~' b" := (BNot b) (in custom com at level 75, right associativity).
+Notation "a //\\ b" := (BAnd a b) (in custom com at level 60, right associativity).
+Notation "a <= b" := (BLessEqual a b) (in custom com at level 60).
 Notation "'~' b" := (BNot b) (in custom com at level 75, right associativity).
 Open Scope com_scope.
 
@@ -58,7 +76,46 @@ Fixpoint aeval (st : state) (a : aexp) : option nat :=
       | Some va1, Some va2 => Some (va1 + va2)
       | _, _ => None
       end
+  | <{a1 - a2}> => match (aeval st a1), (aeval st a2) with
+      | Some va1, Some va2 => Some (va1 - va2)
+      | _, _ => None
+      end
+  | <{a1 * a2}> => match (aeval st a1), (aeval st a2) with
+      | Some va1, Some va2 => Some (va1 * va2)
+      | _, _ => None
+      end
   end.
+
+
+Inductive aevalR : aexp -> nat -> Prop :=
+  | E_ANum (n : nat) :
+      (ANum n) ==> n
+  | E_APlus (e1 e2 : aexp) (n1 n2 : nat) :
+      (e1 ==> n1) ->
+      (e2 ==> n2) ->
+      (APlus e1 e2) ==> (n1 + n2)
+  | E_AMinus (e1 e2 : aexp) (n1 n2 : nat) :
+      (e1 ==> n1) ->
+      (e2 ==> n2) ->
+      (AMinus e1 e2) ==> (n1 - n2)
+  | E_AMult (e1 e2 : aexp) (n1 n2 : nat) :
+      (e1 ==> n1) ->
+      (e2 ==> n2) ->
+      (AMult e1 e2) ==> (n1 * n2)
+  where "e '==>' n" := (aevalR e n) : type_scope.
+
+Definition NOTEQUAL (a1 a2: aexp) : bexp := <{~ (a1 = a2)}>.
+
+Definition GREATEREQUAL (a1 a2: aexp) : bexp := <{ a2 <= a1 }>.
+
+Definition GREATER (a1 a2: aexp) : bexp := <{~ (a1 <= a2)}>.
+
+Definition LESS (a1 a2: aexp) : bexp := GREATER a2 a1.
+
+Definition OR (b1 b2: bexp) : bexp := <{~ ((~ b1) //\\ (~ b2))}>.
+
+Notation "a \\// b" := (OR a b) (in custom com at level 80, right associativity).
+
 
 Definition equal_option [A B] (eq : A -> B -> bool) (a : option A) (b : option B) : bool
   := match a with
@@ -77,8 +134,41 @@ Fixpoint beval (st : state) (b : bexp): bool :=
   | BTrue => true
   | BFalse => false
   | BEq a1 a2 => equal_option (Nat.eqb) (aeval st a1) (aeval st a2)
+  | BLessEqual a1 a2 => equal_option (Nat.leb) (aeval st a1) (aeval st a2)
+  | BAnd b1 b2 => andb (beval st b1) (beval st b2)
   | BNot b1 => negb (beval st b1)
   end.
+
+Lemma beval_OR:
+  forall st b1 b2, beval st <{b1 \\// b2}> = beval st b1 || beval st b2.
+Proof.
+  intros. cbn.
+  rewrite negb_andb.
+  do 2 rewrite negb_involutive.
+  reflexivity.
+Qed.
+
+(*
+  The value of an expression depends only on the values of its free variables.
+
+  Free variables are defined by this recursive predicate:
+*)
+Fixpoint free_in_aexp (x: ident) (a: aexp) : Prop :=
+  match a with
+  | ANum n => False
+  | AId y => y = x
+  | APlus a1 a2 | AMinus a1 a2 | AMult a1 a2 => free_in_aexp x a1 \/ free_in_aexp x a2
+  end.
+
+Theorem aeval_free:
+  forall s1 s2 a,
+  (forall x, free_in_aexp x a -> get s1 x = get s2 x) ->
+  aeval s1 a  = aeval s2 a .
+Proof.
+  induction a; cbn; intros Hfree; auto.
+  all: (rewrite IHa1, IHa2; auto).
+Qed.
+
 
 Reserved  Notation "'assume' l " 
           (in custom com at level 8, l custom com at level 0).
@@ -99,6 +189,9 @@ Notation "x ; y" :=
 Notation "'assume' l " :=
         (Assume l)
           (in custom com at level 8, l custom com at level 0) : com_scope.
+Notation "'nondet' l " :=
+        (Assume l)
+          (in custom com at level 8, l custom com at level 0) : com_scope.
 Notation "'error()'" :=
           Error (in custom com at level 0) : com_scope.
 Notation "c '⋆'" :=
@@ -108,7 +201,7 @@ Notation "x '⨁' y " :=
 
 (* Notations for while, if and assert keywords *)
 
-Definition While b c := <{ (assume b ; c)⋆ ; assume ~ b }>.
+Definition While b c := <{ (assume b ; c) ⋆ ; assume ~ b }>.
 
 Notation "'while' b 'do' c" :=
   (While b c)
@@ -125,22 +218,29 @@ Definition Assert b := <{ (assume b) ⨁ ((assume ~ b) ; error()) }>.
 Notation "'assert' '(' c ')' " :=
   (Assert c) (in custom com at level 8) : com_scope.
 
+Fixpoint Cpow (C: com) (n: nat): com := 
+match n with
+| 0 => <{skip}>
+| S m => <{ C ; Cpow C m }>
+end.
+
+Infix "^" := Cpow (in custom com at level 10).
+
+(* Notation "c '^' n" :=
+  (Cpow c n) (in custom com at level 8) : com_scope. *)
 
 Reserved Notation
          "st '=[' c ']=>' ϵ ':' st'"
          (at level 40, c custom com at level 99,
           st constr, ϵ constr at next level).
 
-
 Inductive Signal: Type := 
 | ok
 | err.
 
 Inductive ceval : com -> state -> Signal -> state -> Prop :=
-| E_Skip : forall st,
-  st =[ skip ]=> ok : st
-| E_SkipF :
-  empty =[ skip ]=> err : empty
+| E_Skip : forall st eps,
+  st =[ skip ]=> eps : st
 | E_Local : forall st st' x v c ϵ,
   (x !-> v ; st) =[ local x . c ]=> ϵ : (x !-> v ; st')
 | E_Asgn : forall st a n x,
@@ -165,10 +265,13 @@ Inductive ceval : com -> state -> Signal -> state -> Prop :=
   empty =[ error() ]=> ok: empty
 | E_Error: forall st,
   st =[ error() ]=> err: st
-| E_StarZero : forall c st ϵ,
+| E_StarSkip : forall c st ϵ,
+  st =[ skip ]=> ϵ : st -> 
   st =[ c ⋆ ]=> ϵ : st
-| E_StarNonZero : forall c st st' ϵ,
-  st =[ c ⋆ ; c  ]=> ϵ : st' ->
+| E_StarIter : forall c st st' ϵ,
+  (* st =[ c ⋆ ; c  ]=> ϵ : st' -> *)
+  st =[ c ⋆ ]=> ϵ : st ->
+  st =[ c ]=> ϵ : st' -> 
   st =[ c ⋆ ]=> ϵ : st'
 | E_ChoiceLeft: forall x y st st' ϵ,
   st =[ x ]=> ϵ : st' ->
@@ -176,10 +279,11 @@ Inductive ceval : com -> state -> Signal -> state -> Prop :=
 | E_ChoiceRight: forall x y st st' ϵ,
   st =[ y ]=> ϵ : st' ->
   st =[ x ⨁ y ]=> ϵ : st'
+(* | E_Nondet: forall x st n,
+  st =[ skip ]=> ok : (x !-> n ; st) *)
 where "st =[ c ]=> ϵ : st'" := (ceval c st ϵ st').
 
 Local Hint Constructors ceval : core.
-
 
 Definition Assertion := state -> Prop.
 
@@ -212,7 +316,6 @@ Notation "P <-> Q" := (fun st => assertion P st <-> assertion Q st) : assertion_
 Notation "a = b" := (fun st => mkAexp a st = mkAexp b st) : assertion_scope.
 Notation "a + b" := (fun st => mkAexp a st + mkAexp b st) : assertion_scope.
 
-
 Definition assert_implies (P Q : Assertion) : Prop :=
   forall st, P st -> Q st.
 
@@ -223,5 +326,82 @@ Notation "P ->> Q" := (assert_implies P Q)
 Open Scope inclogic_spec_scope.
 
 Notation "P <<->> Q" :=
-  (P ->> Q /\ Q ->> P) (at level 80) : inclogic_spec_scope. 
+  (P ->> Q /\ Q ->> P) (at level 80) : inclogic_spec_scope.
 
+
+Hint Unfold assert_implies : core.
+
+
+(* substAexp x y a, which replaces all occurrences of a variable x with a value y inside an arithmetic expression a. *)
+Fixpoint substAexp (x: string) (y: aexp) (a: aexp) : aexp :=
+match a with
+  | ANum n => ANum n
+  | AId var => if String.eqb x var then y else (AId var)
+  | <{a1 + a2}> => <{(substAexp x y a1) + (substAexp x y a2)}>
+  | <{a1 - a2}> => <{(substAexp x y a1) - (substAexp x y a2)}>
+  | <{a1 * a2}> => <{(substAexp x y a1) * (substAexp x y a2)}>
+end.
+
+(* substBeval x y b, which replaces all occurrences of a variable x with a value y inside a boolean expression b. *)
+Fixpoint substBeval (x: string) (y: aexp) (b: bexp) : bexp :=
+let auxa t := substAexp x y t in
+let aux t := substBeval x y t in
+match b with
+| BTrue => BTrue
+| BFalse => BFalse
+| BEq a1 a2 => BEq (auxa a1) (auxa a2)
+| BNot b => aux b
+| <{ a1 <= a2 }> => <{ auxa a1 <= auxa a2 }>
+| <{ b1 //\\ b2 }> => <{(aux b1) //\\ (aux b2)}>
+end.
+
+(* subst x y c, which replaces all occurrences of a variable x with a value y inside a command c. *)
+Fixpoint substCmd (x: string) (y: aexp) (c: com) : com :=
+let aux t := substCmd x y t in
+match y with 
+| AId yvar => 
+  let if_y_eq z t1 t2 := if String.eqb x z then t1 (* update *) else t2 (* skip *) in
+  match c with
+  | Skip => Skip
+  | Asign x' v =>  if_y_eq x' (Asign yvar (substAexp x y v)) (Asign x' (substAexp x y v)) 
+  | Seq c1 c2 => Seq (aux c1) (aux c2) 
+  | Assume b => Assume b
+  | Error => Error
+  | Star c => Star (aux c)
+  | Choice c1 c2 => Choice (aux c1) (aux c2)
+  | CLocal x' c' => if_y_eq x' (CLocal yvar (aux c')) (CLocal x' (aux c'))
+  | Nondet x' => if_y_eq x' (Nondet yvar) (Nondet x')
+  end
+| w => 
+  match c with
+  | Skip => Skip
+  | Asign var exp =>  (Asign var (substAexp x w exp))
+  | Seq c1 c2 => Seq (aux c1) (aux c2) 
+  | Assume b => Assume (substBeval x w b)
+  | Error => Error
+  | Star c => Star (aux c)
+  | Choice c1 c2 => Choice (aux c1) (aux c2)
+  | CLocal x' c' => (CLocal x' (aux c'))
+  | Nondet x' => Nondet x'
+  end
+end.
+
+Example testsubstCmd: substCmd "X"%string (AId "Y"%string)
+  <{ "X" := (AId "X"%string); skip; "Z" :=  (AId "X"%string)}> 
+  = <{ "Y" := (AId "Y"%string); skip; "Z" :=  (AId "Y"%string)}>.
+Proof. reflexivity. Qed.
+
+Example testsubstCmd2: substCmd "X"%string (APlus (ANum 1) (ANum 1))
+  <{ "Y" := (AId "X"%string); skip; "Z" :=  (APlus (ANum 1) (AId "X"%string))}> 
+  = <{ "Y" := (APlus (ANum 1) (ANum 1)); skip; "Z" := (APlus (ANum 1) (APlus (ANum 1) (ANum 1)))}>.
+Proof. reflexivity. Qed.
+
+
+(* - apply (E_Seq_Norm c <{ c ⋆ }> _ _ _ _ H6 H2). *)
+
+(* induction c; inversion H; subst.
+- econstructor. apply H6. *)
+
+
+Hint Unfold assert_implies : core.
+Hint Unfold assert_of_Prop Aexp_of_nat Aexp_of_aexp : core.
