theories/Inc.v
@@ -9,10 +9,8 @@ Require Export Coq.Strings.String.
 From Coq Require Import Lists.List.
 Require Import Ltac2.Option.
 
-Require Import StringAsOT.
 Require Import StateMap.
 Require Import Imp.
-Require Import Hoare.
 
 Import ListNotations.
 
@@ -29,8 +27,15 @@ Notation "[[ P ]] c [[ ϵ ↑ Q ]]" :=
 Notation "[[ P ]] c [[ ok ↑ Q ]] [[ err ↑ R ]] " :=
   ([[ P ]] c [[ ok ↑ Q ]] /\ [[ P ]] c [[ err ↑ R ]]) (at level 90, c custom com at level 99): inclogic_spec_scope.
 
-
 Local Hint Constructors ceval : core.
+
+Hint Unfold assert_implies : core.
+Hint Unfold Inc_triple : core.
+Hint Unfold assert_of_Prop Aexp_of_nat Aexp_of_aexp : core.
+
+(* ========================================== 
+  Generic Proof Rules of Incorrectness Logic
+ ============================================ *)
 
 (*
   [p]C1[ok:q] [q]C2[ϵ:r]
@@ -163,37 +168,6 @@ Proof.
     eauto.
 Qed.
 
-(*
-  ∧∨ Symmetry: [p]c[q1] ∧ [p]c[q2] ⇐⇒ [p]c[q1 ∨ q2]
-               {p}c{q1} ∧ {p}c{q2} ⇐⇒ {p}c{q1 ∧ q2}
-
-*)
-Theorem Inc_sym_and_or: forall P Q1 Q2 ε c,
-  [[ P ]] c [[ ε ↑ Q1 ]] [[ ε ↑ Q2 ]] <-> [[ P ]] c [[ ε ↑ Q1 \/ Q2  ]].
-Proof.
-  intros.
-  split.
-  (* -> *)
-  - intro H.
-    destruct H as [HIncQ1 HIncQ2].
-    intros st' [ HQ1 | HQ2 ].
-    + eapply HIncQ1 ; eauto.
-    + eapply HIncQ2 ; eauto.
-  - (* <- *)
-    intro H.
-    unfold Inc_triple.
-    split.
-    + intros st' H1.
-      apply (discard_disjunction P Q1 Q2 ε c) in H.
-      unfold Inc_triple in H.
-      apply (H st' H1).
-    + intros st' H2.
-      rewrite (Inc_or_comm _ _ _ _ ) in H.
-      apply (discard_disjunction P Q2 Q1 ε c) in H.
-      unfold Inc_triple in H.
-      apply (H st' H2).
-Qed.
-
 (**
  --------------------  (Skip)
       [[ P ]] skip [[ok: P ]] [[er: False ]]
@@ -275,13 +249,19 @@ Qed.
   [p] C⋆ [ε:q]
 *)
 Theorem HInc_IterateNonZero : forall P c ε Q,
-[[ P ]] c ⋆ ; c [[ ε ↑ Q ]] ->
-  [[ P ]] c ⋆ [[ ε ↑ Q ]].
+[[ P ]] (c ⋆) ; c [[ ε ↑ Q ]] ->
+[[ P ]] c ⋆ [[ ε ↑ Q ]].
 Proof.
-  intros P c ε Q HCstarSeq st' HQ.
-  specialize (HCstarSeq st' HQ) as [ st [ Heval HP ] ].
-  inversion Heval; subst; eauto.  
-Qed.
+  (* unfold Inc_triple. *)
+  intros P c ε Q HCstarSeq. 
+  intros st' HQ.
+  specialize (HCstarSeq st').
+  assert (G : exists st : state, st =[ c ⋆; c ]=> ε : st' /\ P st) by auto.
+  destruct G as [ st [Heval HP] ].
+  exists st.
+  split; auto.
+  inversion Heval; subst.
+Abort.
 
 (* FIXME: *)
 (*
@@ -306,40 +286,13 @@ Admitted.
 
 
 
-Reserved Notation "C'^'n" (at level 1, no associativity).
-
-
-Fixpoint Cpow (n: nat) (C: com): com := 
-match n with
-| 0 => <{skip}>
-| S m => <{ C ; Cpow m C }>
-end.
-
 (* FIXME: *)
-Theorem DeriveIteration : forall P c ε Q b,
-  forall x, x < b -> [[ P ]] Cpow x c [[ ε ↑ Q ]] ->
-  [[ P ]] c ⋆ [[ ε ↑ fun st' => x < b -> Q st' ]].
+Theorem DeriveIteration : forall P c ε Q i bound,
+  i <= bound -> [[ P ]] Cpow c i  [[ ε ↑ Q ]] ->
+  [[ P ]] c ⋆ [[ ε ↑ fun st' => forall i, i <= bound -> Q st' ]].
 Proof with auto.
-  (* intros P c ε Q b x H HCstarSeq st HQ.
-  destruct x.
-  - simpl in *. exists st.
-    specialize (HQ H).
-    specialize (HCstarSeq st HQ) as [ st' [ Heval HP ] ].
-    inversion Heval. subst.
-    split...
-  - simpl in *.
-    specialize (HQ H).
-    (* unfold Inc_triple in HCstarSeq. *)
-    pose (HCstarSeq st HQ).
-    destruct e as [ st' [ Heval HP ] ].
-    unfold Inc_triple in HCstarSeq.
-    apply lt_succ_l in H.
-    exists st'.
-
-    admit. *)
-    (* apply IHx H  *)
-  (* specialize (HCstarSeq st' HQ) as [ st [ Heval HP ] ]. *)
-  (* inversion Heval; subst; eauto.   *)
+  intros P c ε Q i bound H_i_leq_bound Hpower.
+  intros st' HQ.
 Admitted.
 
 (*
@@ -368,7 +321,7 @@ Proof with auto.
   - apply Empty_under_approximates.
 Qed.
 
-(*
+(* Alternative
 Theorem inc_asgn : forall X P a,
   [[ fun st' => P st' ]]
     X := a
@@ -430,66 +383,9 @@ Proof with auto.
     exists st2...  
 Qed.
 
-(* substAexp x y a, which replaces all occurrences of a variable x with a value y inside an arithmetic expression a. *)
-Fixpoint substAexp (x: string) (y: aexp) (a: aexp) : aexp :=
-match a with
-  | ANum n => ANum n
-  | AId var => if var_eq x var then y else x
-  | <{a1 + a2}> => <{(substAexp x y a1) + (substAexp x y a2)}>
-end.
-
-(* substBeval x y b, which replaces all occurrences of a variable x with a value y inside a boolean expression b. *)
-Fixpoint substBeval (x: string) (y: aexp) (b: bexp) : bexp :=
-let auxa t := substAexp x y t in
-let aux t := substBeval x y t in
-match b with
-| BTrue => BTrue
-| BFalse => BFalse
-| BEq a1 a2 => BEq (auxa a1) (auxa a2)
-| BNot b => aux b
-end.
-
-(* subst x y c, which replaces all occurrences of a variable x with a value y inside a command c. *)
-Fixpoint substCmd (x: string) (y: aexp) (c: com) : com :=
-let aux t := substCmd x y t in
-match y with 
-| AId yvar => 
-  let if_y_eq z t1 t2 := if var_eq x z then t1 (* change nothing *) else t2 (* update *) in
-  match c with
-  | Skip => Skip
-  | Asign x' v =>  if_y_eq x' (Asign yvar (substAexp x y v)) (Asign x' (substAexp x y v)) 
-  | Seq c1 c2 => Seq (aux c1) (aux c2) 
-  | Assume b => Assume b
-  | Error => Error
-  | Star c => Star (aux c)
-  | Choice c1 c2 => Choice (aux c1) (aux c2)
-  | CLocal x' c' => if_y_eq x' (CLocal yvar (aux c')) (CLocal x' (aux c'))
-  end
-| w => 
-  match c with
-  | Skip => Skip
-  | Asign var exp =>  (Asign var (substAexp x w exp))
-  | Seq c1 c2 => Seq (aux c1) (aux c2) 
-  | Assume b => Assume (substBeval x w b)
-  | Error => Error
-  | Star c => Star (aux c)
-  | Choice c1 c2 => Choice (aux c1) (aux c2)
-  | CLocal x' c' => (CLocal x' (aux c'))
-  end
-end.
-
-Example testsubstCmd: substCmd "X"%string (AId "Y"%string)
-  <{ "X" := (AId "X"%string); skip; "Z" :=  (AId "X"%string)}> 
-  = <{ "Y" := (AId "Y"%string); skip; "Z" :=  (AId "Y"%string)}>.
-Proof. reflexivity. Qed.
-
-
-Example testsubstCmd2: substCmd "X"%string (APlus (ANum 1) (ANum 1))
-  <{ "Y" := (AId "X"%string); skip; "Z" :=  (APlus (ANum 1) (AId "X"%string))}> 
-  = <{ "Y" := (APlus (ANum 1) (ANum 1)); skip; "Z" := (APlus (ANum 1) (APlus (ANum 1) (ANum 1)))}>.
-Proof. reflexivity. Qed.
-
-
+(* ========================================== 
+  Rules for Variables and Mutation
+ ============================================ *)
 
 (* Local Variable
 
@@ -497,12 +393,12 @@ Proof. reflexivity. Qed.
   ------------------------- y ∈ Free(p, C)  
   [p] local x. C [ε: ∃y. q]
 *)
-Theorem LocalVariable : forall P Q F (C: com) (y: aexp) (x: string) ε,
+(* Theorem LocalVariable : forall P Q F (C: com) (y: aexp) (x: string) ε,
   [[ P ]] substCmd x y C [[ ε ↑ Q ]]
   ->
   [[ P /\ F ]] local x . C [[ ε ↑ Q /\ F ]].
 Proof.
-Admitted.
+Admitted. *)
 
 (* x is free in p if p is invariant under changing x
   : i.e., σ ∈ p ⇔ ∀ v. (σ | x ↦ v) ∈ p, where (σ | x ↦ v) for the 
@@ -510,21 +406,21 @@ Admitted.
 *)
 Definition Free x p : Prop := forall st, p st -> forall v, p (x !-> v ; st) .
 
-Module FsetString := FSetList.Make(String_as_OT). 
+(* Module FsetString := FSetList.Make(String_as_OT).  *)
 
 (* Mod(C) is the set of variables modified by assignment statements in C *)
-Fixpoint Mod (c: com): FsetString.t :=
+(* Fixpoint Mod (c: com): FsetString.t :=
 match c with 
 | Asign s a => FsetString.singleton s
 | Seq c1 c2 => FsetString.union (Mod c1) (Mod c2) 
 | _ => FsetString.empty
-end.
+end. *)
 
-Example ModTest1 : FsetString.elements (Mod <{ "X" := 1 ; skip ; "Y" := 2  }>)  = [ "X"%string ; "Y"%string ].
+(* Example ModTest1 : FsetString.elements (Mod <{ "X" := 1 ; skip ; "Y" := 2  }>)  = [ "X"%string ; "Y"%string ].
 Proof. reflexivity. Qed.
 
 Example ModTest2 : FsetString.elements (Mod <{ "X" := 1  }>)  = [ "X"%string ].
-Proof. reflexivity. Qed.
+Proof. reflexivity. Qed. *)
 
 (* The rules of Substitution and Constancy, as well as Consequence, are important for adapting
 specifications for use in different contexts *)
@@ -567,52 +463,59 @@ Theorem Subst2 : forall P Q c ε y x,
 Proof.
 Admitted.
 
-(*  Local BEGIN VAR V1; · · · VAR Vn; C END
-  Semantics: command C is executed, then the values of V1, · · · , Vn
-  are restored to the values they had before the block was entered
+
+(* ========================================== 
+  Connection Incorrectness logic and Partial Correctness logic
+  [P] c [Q] ⊆  post(c) ⊆ {P} c {Q}
+ ============================================ *)
+
+Section IncToCorrection.
+
+(*
+  ∧∨ Symmetry: [p]c[q1] ∧ [p]c[q2] ⇐⇒ [p]c[q1 ∨ q2]
+               {p}c{q1} ∧ {p}c{q2} ⇐⇒ {p}c{q1 ∧ q2}
 
 *)
-Definition W : string := "W".
-Definition X : string := "X".
-Definition Y : string := "Y".
-Definition Z : string := "Z".
+Theorem Inc_sym_and_or: forall P Q1 Q2 ε c,
+  [[ P ]] c [[ ε ↑ Q1 ]] [[ ε ↑ Q2 ]] <-> [[ P ]] c [[ ε ↑ Q1 \/ Q2  ]].
+Proof.
+  intros.
+  split.
+  (* -> *)
+  - intro H.
+    destruct H as [HIncQ1 HIncQ2].
+    intros st' [ HQ1 | HQ2 ].
+    + eapply HIncQ1 ; eauto.
+    + eapply HIncQ2 ; eauto.
+  - (* <- *)
+    intro H.
+    unfold Inc_triple.
+    split.
+    + intros st' H1.
+      apply (discard_disjunction P Q1 Q2 ε c) in H.
+      unfold Inc_triple in H.
+      apply (H st' H1).
+    + intros st' H2.
+      rewrite (Inc_or_comm _ _ _ _ ) in H.
+      apply (discard_disjunction P Q2 Q1 ε c) in H.
+      unfold Inc_triple in H.
+      apply (H st' H2).
+Qed.
 
-
-(* weakest under-approximate post 
-  It is similar to the Hoare Strongest Postconditions
-  If {P} S {Q} and for all Q’ such that {P} S {Q’}, Q ⇒ Q’, then Q is the strongest postcondition of S with respect to P
-
-  - StrongestOverPost(r)p = ⋀ {q | {p}r{q} holds}
-  - WeakestUnderPost(r)p = ⋁ {q | [p]r[q] holds}
-
-  Proposition 8. StrongestOverPost(r) = WeakestUnderPost(r) = post(r)
-  NOTE: we define the n-ary disjunction ⋁ {q | φ q } by `exists`
-*)
-Definition wpp P c Q ε :=
-  [[ P ]] c [[ ε ↑ Q ]] /\
-  exists Q', [[ P ]] c [[ ε ↑ Q' ]] -> (Q ->> Q').
-
-
-(* TODO: Make a more concrete example to challenge wpp *)
-Example is_wpp: wpp (fun st => True) <{ skip }> (fun st => True) ok. 
-Admitted.
-
-Declare Scope hoare_spec_scope.
-
-Open Scope hoare_spec_scope.
+(* FIXME:  *)
 
 (* Principle of Agreement : [u]c[u'] ∧ u ⇒ o ∧ {o}c{o'} ⇒ u' => o' *)
-Lemma Agreement: forall IPRe IPost c ε HPre HPost, [[IPRe]] c [[ ε ↑ IPost ]] /\ IPRe ->> HPre /\ (hoare_triple HPre c ε HPost) -> IPost ->> HPost.
+(* Lemma Agreement: forall IPRe IPost c ε HPre HPost, [[IPRe]] c [[ ε ↑ IPost ]] /\ IPRe ->> HPre /\ (hoare_triple HPre c ε HPost) -> IPost ->> HPost.
 Proof.
   intros IPRe IPost c ε HPre HPost [ HTripleInc [ HyIPReimpHPre HTripleHoare ] ] st' HIpost.
   apply HTripleInc in HIpost.
-  destruct HIpost as [ st [ HInceval HIPre ] ].
+  destruct HIpost as [ st [ HIncEval HIPre ] ].
   apply HyIPReimpHPre in HIPre.
   eapply HTripleHoare in HIPre; eauto.
-Qed.
+Qed. *)
 
 (* Principle of Denial: [u]c[u'] ∧ u ⇒ o ∧ ¬(u' ⇒ o') ⇒ ¬({o}c{o'}) *)
-Lemma Denial: forall IPRe IPost c ε HPre HPost, [[IPRe]] c [[ ε ↑ IPost ]] /\ IPRe ->> HPre /\ ~(IPost ->> HPost) ->  ~(hoare_triple HPre c ε HPost).
+(* Lemma Denial: forall IPRe IPost c ε HPre HPost, [[IPRe]] c [[ ε ↑ IPost ]] /\ IPRe ->> HPre /\ ~(IPost ->> HPost) ->  ~(hoare_triple HPre c ε HPost).
 Proof.
   intros IPRe IPost c ε HPre HPost [ HTripleInc [ HyIPReimpHPre HnotIPostimpHpost ] ] HTripleHoare.
   apply HnotIPostimpHpost.
@@ -622,4 +525,59 @@ Proof.
   destruct HIpost as [ st [ HInceval HIPre ] ].
   apply HyIPReimpHPre in HIPre.
   eapply HTripleHoare in HIPre; eauto.
+Qed. *)
+
+End IncToCorrection.
+
+(* ========================================== 
+   Predicate Transformers
+ ============================================ *)
+
+Section weakest_under_approximate_post.
+
+(* weakest under-approximate post 
+  It is similar to the Hoare Strongest Postconditions
+  If {P} S {Q} and for all Q’ such that {P} S {Q’}, Q ⇒ Q’, then Q is the strongest postcondition of S with respect to P
+
+  - StrongestOverPost(r)p = ⋀ {q | {p}r{q} holds}
+  - WeakestUnderPost(r)p = ⋁ {q | [p]r[q] holds}
+
+  NOTE: we define the n-ary disjunction ⋁ {q | φ q } by `exists`
+*)
+
+(*   Proposition 8. StrongestOverPost(r) = WeakestUnderPost(r) = post(r) *)
+
+Definition is_wup P c Q ε :=
+  [[ P ]] c [[ ε ↑ Q ]] /\
+  exists Q', [[ P ]] c [[ ε ↑ Q' ]] -> (Q ->> Q').
+
+Example is_wup_skip: forall A ε, is_wup (fun st => A) <{ skip }> (fun st => A) ε.
+Proof.
+intros A eps. unfold is_wup.
+split.
+- intros st Q. exists st. eauto. 
+- exists A. auto.
 Qed.
+
+Definition wup (c: com) (P: Assertion) (e: Signal) : Assertion :=
+  fun st' => exists st, st =[ c ]=> e : st' /\ P st.
+
+Lemma wup_postcondition: forall c P ε, [[ P ]] c [[ ε ↑ (wup c P ε) ]].
+Proof.
+  unfold Inc_triple, wup.
+  intros.
+  destruct H as [st H2].
+  eauto.
+Qed.
+
+Lemma wup_weakest_post: forall P c Q ε, [[ P ]] c [[ ε ↑ Q ]] -> (Q ->> wup c P ε).
+Proof.
+  unfold Inc_triple, wup, "->>".
+  intros.
+  specialize (H st).
+  apply H.
+  assumption.
+Qed.
+
+End weakest_under_approximate_post.
+
