theories/Hoare.v
@@ -1,6 +1,12 @@
-Require Import StringAsOT.
 Require Import StateMap.
 Require Import Imp.
+
+(**
+   We give a semantic interpretation to the statements [Hoare P c Q]
+   of Hoare logic.  The interpretation is the relation [triple P c Q]
+   defined below in terms of IMP's natural semantics
+   (the relation [cexec s c s']).
+*)
 
 Definition hoare_triple
            (P : Assertion) (c : com) (s: Signal) (Q : Assertion) : Prop :=
@@ -11,3 +17,49 @@ Definition hoare_triple
 
 Notation "{{ P }} c {{ ε ↑ Q }}" :=
 (hoare_triple P c ε Q) (at level 90, c custom com at level 99): inclogic_spec_scope.
+
+Theorem hoare_post_true : forall (P Q : Assertion) s c,
+  (forall st, Q st) ->
+  {{ P }} c {{ s ↑ Q }}.
+Proof.
+  unfold hoare_triple. intros. apply H.
+Qed.
+
+Theorem hoare_pre_false : forall (P Q : Assertion) c s,
+  (forall st, ~ (P st)) ->
+  {{ P }} c {{ s ↑ Q }}.
+Proof.
+  unfold hoare_triple.
+  intros.
+  apply H in H1. destruct H1.
+Qed.
+
+Theorem hoare_skip : forall P s,
+     {{ P }} skip {{ s ↑ P }}.
+Proof.
+  intros P s st st' H HP.
+  inversion H; subst; assumption.
+Qed.
+
+Theorem hoare_seq : forall P Q R c1 c2 e,
+     {{ Q }} c2 {{ e ↑ R }} ->
+     {{ P }} c1 {{ ok ↑ Q }} ->
+     {{ P }} c1; c2 {{ e ↑ R }}.
+Proof.
+  unfold hoare_triple.
+  intros P Q R c1 c2 e H1 H2 st st'' H12 Pre.
+  specialize (H1 st st'').
+  
+  (* specialize (H2 st st''). *)
+  
+  (* inversion H12; subst.
+  - specialize (H1 st'0 st').
+    apply H1.
+    assumption.
+    specialize (H2 st st'0).
+    eapply H2; 
+    assumption.
+  - specialize (H1 st st').
+    specialize (H2 st st'). *)
+    
+Admitted.
